src/SuperBlock.v
@@ -1,0 +1,203 @@
+Require Import Prog.
+Require Import Word.
+Require Import Rec.
+Require Import List.
+Require Import Pred PredCrash.
+Require Import Eqdep_dec.
+Require Import Arith.
+Require Import Hoare.
+Require Import SepAuto.
+Require Import Cache.
+Require Import AsyncDisk.
+Require Import Omega.
+Require Import FSLayout.
+
+Import ListNotations.
+Set Implicit Arguments.
+
+Module SB.
+
+  Local Hint Resolve goodSize_add_l goodSize_add_r.
+
+  Definition superblock_type : Rec.type := Rec.RecF ([
+      ("data_start",  Rec.WordF addrlen);
+      ("log_header",  Rec.WordF addrlen);
+      ("log_descr",   Rec.WordF addrlen);
+      ("log_descrlen",   Rec.WordF addrlen);
+      ("log_data",    Rec.WordF addrlen);
+      ("log_len",     Rec.WordF addrlen);
+
+      ("ixstart",     Rec.WordF addrlen);
+      ("ixlen",       Rec.WordF addrlen);
+
+      ("bastart",     Rec.WordF addrlen);
+      ("banblocks",   Rec.WordF addrlen);
+
+      ("iastart",     Rec.WordF addrlen);
+      ("ianblocks",   Rec.WordF addrlen);
+
+      ("root_inum",   Rec.WordF addrlen);
+      ("maxblock",    Rec.WordF addrlen)
+    ]).
+
+  Definition superblock_padded : Rec.type := Rec.RecF ([
+      ("sb", superblock_type);
+      ("pad", Rec.WordF (valulen - (Rec.len superblock_type)))
+    ]).
+
+  Theorem superblock_padded_len :
+    Rec.len superblock_padded = valulen.
+  Proof.
+    simpl. rewrite valulen_is. compute. reflexivity.
+  Qed.
+
+  Definition superblock0 := @Rec.of_word superblock_type (wzero _).
+  Definition superblock_pad0 := @Rec.of_word superblock_padded (wzero _).
+
+  Definition pickle_superblock (fsxp : fs_xparams) : word (Rec.len superblock_padded) :=
+    let (lxp, ixp, ibxp, dbxp, rootinum, maxblock) := fsxp in
+    let sb := superblock0
+      :=> "data_start"  := addr2w (DataStart lxp)
+      :=> "log_header"  := addr2w (LogHeader lxp)
+      :=> "log_descr"   := addr2w (LogDescriptor lxp)
+      :=> "log_descrlen":= addr2w (LogDescLen lxp)
+      :=> "log_data"    := addr2w (LogData lxp)
+      :=> "log_len"     := addr2w (LogLen lxp)
+      :=> "ixstart"     := addr2w (IXStart ixp)
+      :=> "ixlen"       := addr2w (IXLen ixp)
+      :=> "bastart"     := addr2w (BmapStart dbxp)
+      :=> "banblocks"   := addr2w (BmapNBlocks dbxp)
+      :=> "iastart"     := addr2w (BmapStart ibxp)
+      :=> "ianblocks"   := addr2w (BmapNBlocks ibxp)
+      :=> "root_inum"   := addr2w rootinum
+      :=> "maxblock"    := addr2w maxblock
+    in Rec.to_word (superblock_pad0 :=> "sb" := sb).
+
+  Definition unpickle_superblock (sbp : word (Rec.len superblock_padded)) : fs_xparams :=
+    let sb := ((Rec.of_word sbp) :-> "sb") in
+    let lxp := Build_log_xparams
+      # (sb :-> "data_start") # (sb :-> "log_header")
+      # (sb :-> "log_descr") # (sb :-> "log_descrlen")
+      # (sb :-> "log_data") # (sb :-> "log_len") in
+    let ixp := Build_inode_xparams
+      # (sb :-> "ixstart") # (sb :-> "ixlen") in
+    let dbxp := Build_balloc_xparams
+      # (sb :-> "bastart") # (sb :-> "banblocks") in
+    let ibxp := Build_balloc_xparams
+      # (sb :-> "iastart") # (sb :-> "ianblocks") in
+    let rootinum := # (sb :-> "root_inum") in
+    let maxblock := # (sb :-> "maxblock") in
+    Build_fs_xparams lxp ixp ibxp dbxp rootinum maxblock.
+
+
+  Theorem pickle_unpickle_superblock : forall fsxp,
+    fs_xparams_ok fsxp ->
+    unpickle_superblock (pickle_superblock fsxp) = fsxp.
+  Proof.
+    unfold pickle_superblock, unpickle_superblock.
+    destruct fsxp.
+    repeat rewrite Rec.of_to_id.
+    destruct FSXPLog.
+    destruct FSXPInode.
+    destruct FSXPInodeAlloc.
+    destruct FSXPBlockAlloc.
+    unfold Rec.recget', Rec.recset'.
+    unfold addr2w; simpl; intros.
+    repeat rewrite wordToNat_natToWord_idempotent' by xparams_ok.
+    auto.
+    unfold Rec.well_formed.
+    simpl.
+    intuition.
+  Qed.
+
+  Definition v_pickle_superblock (fsxp : fs_xparams) : valu.
+    remember (pickle_superblock fsxp) as sb; clear Heqsb.
+    rewrite superblock_padded_len in *.
+    exact sb.
+  Defined.
+
+  Definition v_unpickle_superblock (v : valu) : fs_xparams.
+    rewrite <- superblock_padded_len in *.
+    exact (unpickle_superblock v).
+  Defined.
+
+  Theorem v_pickle_unpickle_superblock : forall fsxp,
+    fs_xparams_ok fsxp ->
+    v_unpickle_superblock (v_pickle_superblock fsxp) = fsxp.
+  Proof.
+    intros.
+    unfold v_pickle_superblock, v_unpickle_superblock.
+    unfold eq_rec_r, eq_rec.
+    rewrite eq_rect_nat_double.
+    rewrite <- (eq_rect_eq_dec eq_nat_dec).
+    apply pickle_unpickle_superblock; auto.
+  Qed.
+
+
+  Definition rep (fsxp : fs_xparams) : rawpred :=
+    ([[ fs_xparams_ok fsxp ]] * 0 |=> v_pickle_superblock fsxp)%pred.
+
+  Definition load T cs rx : prog T :=
+    let^ (cs, v) <- BUFCACHE.read 0 cs;
+    rx ^(cs, v_unpickle_superblock v).
+
+  Theorem load_ok : forall cs,
+    {< m F fsxp,
+    PRE
+      BUFCACHE.rep cs m * [[ (F * rep fsxp)%pred m ]]
+    POST RET:^(cs',r)
+      BUFCACHE.rep cs' m * [[ r = fsxp ]]
+    CRASH
+      exists cs', BUFCACHE.rep cs' m
+    >} load cs.
+  Proof.
+    unfold load, rep.
+    hoare.
+    subst; apply v_pickle_unpickle_superblock; auto.
+  Qed.
+
+  Definition init T fsxp cs rx : prog T :=
+    cs <- BUFCACHE.write 0 (v_pickle_superblock fsxp) cs;
+    cs <- BUFCACHE.sync 0 cs;
+    rx cs.
+
+  Theorem init_ok : forall fsxp cs,
+    {< m F,
+    PRE
+      BUFCACHE.rep cs m * 
+      [[ fs_xparams_ok fsxp /\ (F * 0 |->?)%pred m ]]
+    POST RET:cs
+      exists m',
+      BUFCACHE.rep cs m' * [[ (F * rep fsxp)%pred m' ]]
+    CRASH
+      exists cs' m', BUFCACHE.rep cs' m' * 
+      [[ (F * 0 |->?)%pred m' ]]
+    >} init fsxp cs.
+  Proof.
+    unfold rep, init.
+    hoare.
+  Qed.
+
+  Hint Extern 1 ({{_}} progseq (load _) _) => apply load_ok : prog.
+  Hint Extern 1 ({{_}} progseq (init _ _) _) => apply init_ok : prog.
+
+  Theorem crash_xform_rep : forall fsxp,
+    crash_xform (rep fsxp) <=p=> rep fsxp.
+  Proof.
+    unfold rep; intros; split;
+    rewrite crash_xform_sep_star_dist;
+    rewrite crash_xform_lift_empty.
+
+    rewrite crash_xform_ptsto; cancel.
+    subst; auto.
+
+    rewrite <- crash_xform_ptsto_r.
+    cancel.
+    unfold vsmerge; simpl; auto.
+  Qed.
+
+  Hint Rewrite crash_xform_rep : crash_xform.
+
+  Hint Extern 0 (okToUnify (rep _) (rep _)) => constructor : okToUnify.
+
+End SB.
